\appendix
\section{Further equation}
\begin{equation}
C_{1,ab}=\sqrt{(a_{1})^{2}+(b_{1})^{2}} \quad C_{2,ab}=\sqrt{(a_{2})^{2}+(b_{2})^{2}}
\end{equation}
\begin{equation}
\bar{C}_{ab}=\frac{C_{1,ab}+C_{2,ab}}{2}
\end{equation}
\begin{equation}
G = 0.5(1-\sqrt{\frac{\bar{C}_{ab}^{7}}{\bar{C}_{ab}^{7}+25^7}})
\end{equation}
\begin{equation}
a_{1}'=(1+G)a_{1} \quad a_{2}'=(1+G)a_{2} 
\end{equation}
\begin{equation}
C_{1}'=\sqrt{(a_{1}')^{2}+(b_{1})2} \quad C_{2}'=\sqrt{(a_{2}')^{2}+(b_{2})2}
\end{equation}
\begin{equation}
h_{1}' = atan2(b_{1},a_{1}') =
\begin{cases}
tan^{-1}(\frac{b_{1}}{a_{1}'}) & b_{1}>0,a_{1}' \geq 0\\
tan^{-1}(\frac{b_{1}}{a_{1}'})+180^{\circ} & b_{1}<0\\
tan^{-1}(\frac{b_{1}}{a_{1}'})+360^{\circ} & b_{1}>0,a_{1}'<0 \\
90^{\circ} & b_{1}=0,a_{1}'>0\\
270^{\circ} & b_{1}=0,a_{1}'<0\\
0^{\circ} & b_{1}=0,a_{1}'=0
\end{cases}
\end{equation}
\begin{equation}
h_{2}' = atan2(b_{2},a_{2}') =
\begin{cases}
tan^{-1}(\frac{b_{2}}{a_{2}'}) & b_{2}>0,a_{2}' \geq 0\\
tan^{-1}(\frac{b_{2}}{a_{2}'})+180^{\circ} & b_{2}<0\\
tan^{-1}(\frac{b_{2}}{a_{2}'})+360^{\circ} & b_{2}>0,a_{2}'<0 \\
90^{\circ} & b_{2}=0,a_{2}'>0\\
270^{\circ} & b_{2}=0,a_{2}'<0\\
0^{\circ} & b_{2}=0,a_{2}'=0
\end{cases}
\end{equation}
\begin{equation}
\Delta L'=L_{2}-L_{1}
\end{equation}
\begin{equation}
\Delta C'=C_{2}'-C_{1}'
\end{equation}
\begin{equation}
\Delta h' =
\begin{cases}
0 & C_{1}'C_{2}'=0\\
h_{2}'-h_{1}' & C_{1}'C_{2}'\ne q0, |h_{2}'-h_{1}'| \geq -180^{\circ}\\
(h_{2}'-h_{1}')-360^{\circ} & C_{1}'C_{2}'\neq 0, (h_{2}'-h_{1}') > -180^{\circ}\\
(h_{2}'-h_{1}')+360^{\circ} & C_{1}'C_{2}'\neq 0, (h_{2}'-h_{1}') < -180^{\circ}
\end{cases}
\end{equation}
\begin{equation}
\Delta H'=2\sqrt{C_{1}'C_{2}'}sin(\frac{\Delta h'}{2})
\end{equation}
\begin{equation}
\bar{L}'=\frac{L_{1}+L_{2}}{2}
\end{equation}
\begin{equation}
\bar{C}'=\frac{C_{1}'+C_{2}'}{2}
\end{equation}
\begin{equation}
\bar{h'} =
\begin{cases}
\frac{h_{1}'+h_{2}'}{2} & C_{1}'C_{2}'\neq 0 \wedge |h_{2}'-h_{1}'| \leq 180^{\circ}\\
\frac{h_{1}'+h_{2}'+360^{\circ}}{2}& |h_{2}'-h_{1}'| > 180^{\circ} \wedge (h_{2}'-h_{1}') < 180^{\circ}\\
\frac{h_{1}'+h_{2}'-360^{\circ}}{2} & |h_{2}'-h_{1}'| > 180^{\circ} \wedge (h_{2}'-h_{1}') \geq 360^{\circ}\\
h_{1}'+h_{2}' & C_{1}'C_{2}'=0
\end{cases}
\end{equation}
\begin{equation}
T=1-0.17 cos(\bar{h}'-30^{\circ})+0.24 cos(2\bar{h}')+0.32(3\bar{h}'+6^{\circ})-0.2 cos(4\bar{h}'-63^{\circ})
\end{equation}
\begin{equation}
\Delta 0 = 30e^{-(\frac{h'-275^{\circ}}{25})^{2}}
\end{equation}
\begin{equation}
R_{c}=2\sqrt{\frac{\bar{C'}_{ab}^{7}}{\bar{C'}_{ab}^{7}+25^{7}}}
\end{equation}
\begin{equation}
S_{L}=1+\frac{0.015(\bar{L}'-50)^{2}}{\sqrt{20+(\bar{L}'-50)^{2}}}
\end{equation}
\begin{equation}
S_{C}=1+0.0045\bar{C}'
\end{equation}
\begin{equation}
S_{H}=1+0.0045\bar{C}'T
\end{equation}
\begin{equation}
R_{T}=-sin(2 \Delta 0)R_{c}
\end{equation}